src/Compilers/MapBaseTypeWf.v
@@ -7,7 +7,9 @@ Require Import Crypto.Compilers.ExprInversion.
 Require Import Crypto.Compilers.MapBaseType.
 Require Import Crypto.Util.Tactics.BreakMatch.
 Require Import Crypto.Util.Tactics.DestructHead.
+Require Import Crypto.Util.Tactics.SpecializeBy.
 Require Import Crypto.Util.Sigma.
+Require Import Crypto.Util.Option.
 Require Import Crypto.Util.Prod.
 
 Section language.
@@ -15,8 +17,9 @@ Section language.
           {op1 : flat_type base_type_code1 -> flat_type base_type_code1 -> Type}
           {op2 : flat_type base_type_code2 -> flat_type base_type_code2 -> Type}
           (f_base : base_type_code1 -> base_type_code2)
-          (f_op : forall s d,
+          (f_op : forall var1 s d,
               op1 s d
+              -> exprf _ op1 (var:=var1) s
               -> option (op2 (lift_flat_type f_base s) (lift_flat_type f_base d))).
 
   Local Hint Constructors wf wff or.
@@ -36,6 +39,9 @@ Section language.
             (failb : forall t, exprf _ op2 (var:=var2) (Tbase t))
             (failb' : forall t, exprf _ op2 (var:=var2') (Tbase t))
             (Hwf_failb : forall t G, wff G (failb t) (failb' t))
+            (Hwf_f_op : forall G s d opc e1 e2,
+                wff G e1 e2
+                -> f_op var1 s d opc e1 = f_op var1' s d opc e2)
             (Hvar12 : forall t v, f_var12 t (f_var21 t v) = v)
             (Hvar'12 : forall t v, f_var'12 t (f_var'21 t v) = v).
 
@@ -53,12 +59,17 @@ Section language.
       revert dependent G'; induction Hwf;
         repeat first [ progress simpl in *
                      | progress intros
+                     | progress inversion_option
+                     | progress subst
                      | break_innermost_match_step
+                     | progress specialize_by_assumption
                      | apply wff_SmartPairf_SmartValf
                      | solve [ eauto using In_flatten_binding_list_untransfer_interp_flat_type ]
                      | match goal with
                        | [ |- wff _ _ _ ] => constructor
                        | [ H : _ |- _ ] => apply H; try setoid_rewrite List.in_app_iff
+                       | [ H : f_op _ ?s ?d ?opc ?e = ?x, H' : f_op _ ?s ?d ?opc ?e' = ?y |- _ ]
+                         => assert (x = y) by (rewrite <- H, <- H'; eauto); clear H'
                        end
                      | progress destruct_head'_or ].
     Qed.
@@ -77,15 +88,30 @@ Section language.
     Qed.
   End with_var.
 
-  Lemma Wf_MapBaseType
-        (failb : forall var t, exprf _ op2 (var:=var) (Tbase t))
-        (Hwf_failb : forall var1 var2 G t, wff G (failb var1 t) (failb var2 t))
-        {t} (e : Expr base_type_code1 op1 t)
-        (Hwf : Wf e)
-    : Wf (MapBaseType f_base f_op failb e).
-  Proof using Type.
-    intros var1 var2; apply wf_map_base_type; eauto.
-  Qed.
+  Section MapBaseType.
+    Context (failb : forall var t, exprf _ op2 (var:=var) (Tbase t))
+            (Hwf_failb : forall var1 var2 G t, wff G (failb var1 t) (failb var2 t))
+            (Hwf_f_op : forall var1 var1' s d opc G e1 e2,
+                wff G e1 e2
+                -> f_op var1 s d opc e1 = f_op var1' s d opc e2)
+            {t} (e : Expr base_type_code1 op1 t)
+            (Hwf : Wf e).
+
+    Lemma Wf_MapBaseType'
+      : Wf (MapBaseType' f_base f_op failb e).
+    Proof using Hwf Hwf_failb Hwf_f_op.
+      intros var1 var2; apply wf_map_base_type; eauto.
+    Qed.
+
+    Lemma Wf_MapBaseType
+          r
+          (H : MapBaseType f_base f_op failb e = Some r)
+      : Wf r.
+    Proof using Hwf Hwf_failb Hwf_f_op.
+      cbv [MapBaseType] in *; break_innermost_match_hyps; inversion_option; subst.
+      apply Wf_MapBaseType'.
+    Qed.
+  End MapBaseType.
 End language.
 
-Hint Resolve @Wf_MapBaseType : wf.
+Hint Resolve @Wf_MapBaseType' : wf.
